handling return value of rfm

_build/default/src/proofs/funcall/generated_proof_foo.v.d
@@ -1,0 +1,2 @@
+generated_proof_foo.vo generated_proof_foo.glob generated_proof_foo.v.beautified generated_proof_foo.required_vo: generated_proof_foo.v ./generated_code.vo ./generated_spec.vo
+generated_proof_foo.vio: generated_proof_foo.v ./generated_code.vio ./generated_spec.vio
