_build/default/src/proofs/funcall/generated_spec.v.d
@@ -1,0 +1,2 @@
+generated_spec.vo generated_spec.glob generated_spec.v.beautified generated_spec.required_vo: generated_spec.v ./generated_code.vo
+generated_spec.vio: generated_spec.v ./generated_code.vio
