src/funcall.c
@@ -1,0 +1,42 @@
+#include <stdint.h>
+#include <stdlib.h>
+#include <stdbool.h>
+
+
+// [[rc::exists("value : nat")]]
+// [[rc::returns("value @ int<u8>")]]
+//  uint8_t nondent() { return 2; /* need to return something for proof to work */ }
+
+// [[rc::exists("value : nat")]]
+// [[rc::exists("nondent_value : nat")]]
+// [[rc::returns("value @ int<size_t>")]]
+// [[rc::ensures("{if (Nat.eqb nondent_value 2%nat) then value = 1%nat else value = 2%nat}")]]
+// size_t use_nondent(){
+//     if(nondent() == 2){
+//         return 2;
+//     }
+//     return 1;
+// }
+[[rc::exists("v : bool")]]
+[[rc::returns("v @ builtin_boolean")]]
+ bool nondent() { return 2;}
+
+[[rc::exists("v : Z")]]
+[[rc::returns("v @ int<i32>")]]
+[[rc::ensures("{\exsits w, w = 2 -> v = 1}")]]
+int foo(){
+    if(nondent() == 2){
+        return 1;
+    }
+    return 2;
+}
+
+// [[rc::exists("value : bool")]]
+// [[rc::returns("value @ builtin_boolean")]]
+// [[rc::ensures("{Is_true value}")]]
+// bool example_return(){
+//     // if(nondent() == 2){
+//     //     return 1;
+//     // }
+//     return 1;
+// }
