src/solswitch.c
@@ -10,19 +10,26 @@ SolenoidSwitchingParams_t{
     size_t msg;
 } SolenoidSwitchingParams_t;
 
+//@rc::inlined
+//@Definition SCH_recieveFullMsg_ret (b : nat) : iProp Σ. Admitted. (* TODO: Fill in something here.*)
+//@rc::end
 
 [[rc::parameters("state: nat", "msg: nat", "p: loc")]]
 [[rc::args("p @ &own<{state, msg} @ SolenoidSwitchingParams_t>")]]
 [[rc::exists("new_msg : nat")]]
+[[rc::exists("new_msg_size : nat")]]
+[[rc::returns("new_msg_size @ int<u8>")]]
 [[rc::ensures("own p : {state,new_msg} @ SolenoidSwitchingParams_t")]]
- uint8_t SCH_recieveFullMsg(SolenoidSwitchingParams_t* ssp) 
- {
-
- }
+ uint8_t SCH_recieveFullMsg(SolenoidSwitchingParams_t* ssp) { return 2; /* need to return something for proof to work */ }
 
 [[rc::parameters("state: nat", "msg: nat", "p: loc")]]
 [[rc::args("p @ &own<{state, msg} @ SolenoidSwitchingParams_t>")]]
-[[rc::ensures("own p : { (if Nat.eqb state 0%nat then 1%nat else state) ,msg} @ SolenoidSwitchingParams_t")]]
+[[rc::exists("new_state : nat")]]
+// [[rc::ensures("own p : { (if Nat.eqb state 0%nat then 1%nat else state) ,msg} @ SolenoidSwitchingParams_t")]]
+[[rc::ensures("own p : { new_state ,msg} @ SolenoidSwitchingParams_t")]]
+[[rc::ensures("{new_state = (if Nat.eqb state 0%nat then 1%nat else state)}")]]
+// [[rc::ensures("{state = 0%nat} @ optional<1%nat,state> @ new_state")]]
+// [[rc::ensures("own p : {state = 0%nat} @ optional<{1%nat,msg} @ SolenoidSwitchingParams_t ,{state,msg} @ SolenoidSwitchingParams_t>")]]
 [[rc::tactics("all: try destruct state. try lia. try auto.")]]
 void SML_switchTheSolenoid( SolenoidSwitchingParams_t* ssp){
 
@@ -32,16 +39,64 @@ void SML_switchTheSolenoid( SolenoidSwitchingParams_t* ssp){
 	}
 }
 
-#define UNIQUE_MSG 8
+
+#define INVALID_MSG_SIZE 0
+#define UNIQUE_MSG_SIZE 8
+#define UNIQUE_MSG_A 7
+#define UNIQUE_MSG_B 12
 [[rc::parameters("state: nat", "msg: nat", "p: loc")]]
 [[rc::args("p @ &own<{state, msg} @ SolenoidSwitchingParams_t>")]]
 [[rc::exists("new_msg : nat")]]
-[[rc::exists("new_state : nat")]] // todo - remove this. fix postcondition.
+[[rc::exists("new_state : nat")]]
+[[rc::exists("new_msg_size : nat")]]
+// [[rc::ensures("own p : { (if Nat.eqb new_msg_size 8%nat then 1%nat else state) ,new_msg} @ SolenoidSwitchingParams_t")]]
+// [[rc::ensures("{((new_msg_size = 8%nat)) -> new_state = 1%nat}")]]
+// [[rc::ensures("[SCH_recieveFullMsg_ret (if new_state is 1%nat then 8%nat else 0%nat)]")]]
 [[rc::ensures("own p : { new_state ,new_msg} @ SolenoidSwitchingParams_t")]]
+//[[rc::ensures("{(new_msg_size = 8%nat) -> (new_state = 1%nat)}")]]
+// [[rc::ensures("{∃ n, (and (new_msg_size = n) (n <> 8%nat)) -> new_state = state}")]]
+[[rc::ensures("{∃ len, or ((len = 8%nat) -> (new_state = 1%nat)) ((len <> 8%nat) -> (new_state = state))}")]]
+[[rc::tactics("exists 8%nat. left. auto." )]]
+[[rc::tactics("exists 0%nat. right. auto. " )]]
+[[rc::tactics("exists 0%nat. right. auto. " )]]
 void SML_handleReceivedMsgs(SolenoidSwitchingParams_t* ssp)
 {
-    SCH_recieveFullMsg(ssp);
-    if(ssp->msg == UNIQUE_MSG){
-        SML_switchTheSolenoid(ssp);
+    uint8_t rxMsgSize = SCH_recieveFullMsg(ssp);
+    if(rxMsgSize != INVALID_MSG_SIZE){
+        if(rxMsgSize == UNIQUE_MSG_SIZE){
+            //if(ssp->msg == UNIQUE_MSG_A /*|| ssp->msg == UNIQUE_MSG_B*/){ // todo - msg should be array. not supported in refinedc?
+               //SML_switchTheSolenoid(ssp);
+            //}
+            ssp->state = 1;
+        }
     }
+    
 }
+
+// [[rc::parameters("state: nat", "msg: nat", "p: loc", "len: nat")]]
+// [[rc::args("p @ &own<{state, msg} @ SolenoidSwitchingParams_t>", "len @ int<u8>")]]
+// [[rc::exists("new_msg : nat")]]
+// [[rc::exists("new_state : nat")]]
+// [[rc::ensures("own p : { new_state ,new_msg} @ SolenoidSwitchingParams_t")]]
+// [[rc::ensures("{or (and (len = 8%nat) (new_state = 1%nat)) (and (len <> 8%nat) (new_state = state))}")]]
+// //[[rc::ensures("{new_state = 1%nat ∨ new_state = state}")]]
+// void SML_handleReceivedMsgs_with_length(SolenoidSwitchingParams_t* ssp, uint8_t rxMsgSize)
+// {
+//     // if(rxMsgSize != INVALID_MSG_SIZE){
+//         if(rxMsgSize == UNIQUE_MSG_SIZE){
+//             //if(ssp->msg == UNIQUE_MSG_A /*|| ssp->msg == UNIQUE_MSG_B*/){ // todo - msg should be array. not supported in refinedc?
+//                //SML_switchTheSolenoid(ssp);
+//             //}
+//             ssp->state = 1;
+//         }
+//     // }
+    
+// }
+
+
+
+// void SML_handleReceivedMsgs(SolenoidSwitchingParams_t* ssp)
+// {
+//     uint8_t rxMsgSize = SCH_recieveFullMsg(ssp);
+//     SML_handleReceivedMsgs_with_length(ssp, rxMsgSize);
+// }
