_build/default/src/proofs/solswitch/generated_code.v
@@ -6,39 +6,47 @@ Set Default Proof Using "Type".
 (* Generated from [src/solswitch.c]. *)
 Section code.
   Definition file_0 : string := "src/solswitch.c".
-  Definition loc_4 : location_info := LocationInfo file_0 29 1 32 2.
-  Definition loc_5 : location_info := LocationInfo file_0 29 23 32 2.
-  Definition loc_6 : location_info := LocationInfo file_0 31 2 31 17.
-  Definition loc_7 : location_info := LocationInfo file_0 31 2 31 12.
-  Definition loc_8 : location_info := LocationInfo file_0 31 2 31 5.
-  Definition loc_9 : location_info := LocationInfo file_0 31 2 31 5.
-  Definition loc_10 : location_info := LocationInfo file_0 31 15 31 16.
-  Definition loc_11 : location_info := LocationInfo file_0 29 1 32 2.
-  Definition loc_12 : location_info := LocationInfo file_0 29 6 29 21.
-  Definition loc_13 : location_info := LocationInfo file_0 29 6 29 7.
-  Definition loc_14 : location_info := LocationInfo file_0 29 11 29 21.
-  Definition loc_15 : location_info := LocationInfo file_0 29 11 29 21.
-  Definition loc_16 : location_info := LocationInfo file_0 29 11 29 14.
-  Definition loc_17 : location_info := LocationInfo file_0 29 11 29 14.
-  Definition loc_20 : location_info := LocationInfo file_0 43 4 43 28.
-  Definition loc_21 : location_info := LocationInfo file_0 44 4 46 5.
-  Definition loc_22 : location_info := LocationInfo file_0 44 21 46 5.
-  Definition loc_23 : location_info := LocationInfo file_0 45 8 45 35.
-  Definition loc_24 : location_info := LocationInfo file_0 45 8 45 29.
-  Definition loc_25 : location_info := LocationInfo file_0 45 8 45 29.
-  Definition loc_26 : location_info := LocationInfo file_0 45 30 45 33.
-  Definition loc_27 : location_info := LocationInfo file_0 45 30 45 33.
-  Definition loc_28 : location_info := LocationInfo file_0 44 4 46 5.
-  Definition loc_29 : location_info := LocationInfo file_0 44 7 44 20.
-  Definition loc_30 : location_info := LocationInfo file_0 44 7 44 15.
-  Definition loc_31 : location_info := LocationInfo file_0 44 7 44 15.
-  Definition loc_32 : location_info := LocationInfo file_0 44 7 44 10.
-  Definition loc_33 : location_info := LocationInfo file_0 44 7 44 10.
-  Definition loc_34 : location_info := LocationInfo file_0 44 19 44 20.
-  Definition loc_35 : location_info := LocationInfo file_0 43 4 43 22.
-  Definition loc_36 : location_info := LocationInfo file_0 43 4 43 22.
-  Definition loc_37 : location_info := LocationInfo file_0 43 23 43 26.
-  Definition loc_38 : location_info := LocationInfo file_0 43 23 43 26.
+  Definition loc_2 : location_info := LocationInfo file_0 23 62 23 71.
+  Definition loc_3 : location_info := LocationInfo file_0 23 69 23 70.
+  Definition loc_6 : location_info := LocationInfo file_0 36 1 39 2.
+  Definition loc_7 : location_info := LocationInfo file_0 36 23 39 2.
+  Definition loc_8 : location_info := LocationInfo file_0 38 2 38 17.
+  Definition loc_9 : location_info := LocationInfo file_0 38 2 38 12.
+  Definition loc_10 : location_info := LocationInfo file_0 38 2 38 5.
+  Definition loc_11 : location_info := LocationInfo file_0 38 2 38 5.
+  Definition loc_12 : location_info := LocationInfo file_0 38 15 38 16.
+  Definition loc_13 : location_info := LocationInfo file_0 36 1 39 2.
+  Definition loc_14 : location_info := LocationInfo file_0 36 6 36 21.
+  Definition loc_15 : location_info := LocationInfo file_0 36 6 36 7.
+  Definition loc_16 : location_info := LocationInfo file_0 36 11 36 21.
+  Definition loc_17 : location_info := LocationInfo file_0 36 11 36 21.
+  Definition loc_18 : location_info := LocationInfo file_0 36 11 36 14.
+  Definition loc_19 : location_info := LocationInfo file_0 36 11 36 14.
+  Definition loc_22 : location_info := LocationInfo file_0 64 4 64 48.
+  Definition loc_23 : location_info := LocationInfo file_0 65 4 72 5.
+  Definition loc_24 : location_info := LocationInfo file_0 65 22 72 5.
+  Definition loc_25 : location_info := LocationInfo file_0 66 8 71 9.
+  Definition loc_26 : location_info := LocationInfo file_0 66 26 71 9.
+  Definition loc_27 : location_info := LocationInfo file_0 70 12 70 27.
+  Definition loc_28 : location_info := LocationInfo file_0 70 12 70 22.
+  Definition loc_29 : location_info := LocationInfo file_0 70 12 70 15.
+  Definition loc_30 : location_info := LocationInfo file_0 70 12 70 15.
+  Definition loc_31 : location_info := LocationInfo file_0 70 25 70 26.
+  Definition loc_32 : location_info := LocationInfo file_0 66 8 71 9.
+  Definition loc_33 : location_info := LocationInfo file_0 66 11 66 25.
+  Definition loc_34 : location_info := LocationInfo file_0 66 11 66 20.
+  Definition loc_35 : location_info := LocationInfo file_0 66 11 66 20.
+  Definition loc_36 : location_info := LocationInfo file_0 66 24 66 25.
+  Definition loc_37 : location_info := LocationInfo file_0 65 4 72 5.
+  Definition loc_38 : location_info := LocationInfo file_0 65 7 65 21.
+  Definition loc_39 : location_info := LocationInfo file_0 65 7 65 16.
+  Definition loc_40 : location_info := LocationInfo file_0 65 7 65 16.
+  Definition loc_41 : location_info := LocationInfo file_0 65 20 65 21.
+  Definition loc_42 : location_info := LocationInfo file_0 64 24 64 47.
+  Definition loc_43 : location_info := LocationInfo file_0 64 24 64 42.
+  Definition loc_44 : location_info := LocationInfo file_0 64 24 64 42.
+  Definition loc_45 : location_info := LocationInfo file_0 64 43 64 46.
+  Definition loc_46 : location_info := LocationInfo file_0 64 43 64 46.
 
   (* Definition of struct [div]. *)
   Program Definition struct_div := {|
@@ -86,7 +94,8 @@ Section code.
     f_init := "#0";
     f_code := (
       <[ "#0" :=
-        Return (VOID)
+        locinfo: loc_2 ;
+        Return (LocInfoE loc_3 (UnOp (CastOp $ IntOp u8) (IntOp i32) (LocInfoE loc_3 (i2v 2 i32))))
       ]> $∅
     )%E
   |}.
@@ -101,18 +110,18 @@ Section code.
     f_init := "#0";
     f_code := (
       <[ "#0" :=
-        locinfo: loc_12 ;
-        if{IntOp i32}: LocInfoE loc_12 ((LocInfoE loc_13 (UnOp (CastOp $ IntOp size_t) (IntOp i32) (LocInfoE loc_13 (i2v 0 i32)))) ={IntOp size_t, IntOp size_t, i32} (LocInfoE loc_14 (use{IntOp size_t} (LocInfoE loc_15 ((LocInfoE loc_16 (!{PtrOp} (LocInfoE loc_17 ("ssp")))) at{struct_SolenoidSwitchingParams_t} "state")))))
+        locinfo: loc_14 ;
+        if{IntOp i32}: LocInfoE loc_14 ((LocInfoE loc_15 (UnOp (CastOp $ IntOp size_t) (IntOp i32) (LocInfoE loc_15 (i2v 0 i32)))) ={IntOp size_t, IntOp size_t, i32} (LocInfoE loc_16 (use{IntOp size_t} (LocInfoE loc_17 ((LocInfoE loc_18 (!{PtrOp} (LocInfoE loc_19 ("ssp")))) at{struct_SolenoidSwitchingParams_t} "state")))))
         then
-        locinfo: loc_6 ;
+        locinfo: loc_8 ;
           Goto "#1"
         else
         Goto "#2"
       ]> $
       <[ "#1" :=
-        locinfo: loc_6 ;
-        LocInfoE loc_7 ((LocInfoE loc_8 (!{PtrOp} (LocInfoE loc_9 ("ssp")))) at{struct_SolenoidSwitchingParams_t} "state") <-{ IntOp size_t }
-          LocInfoE loc_10 (UnOp (CastOp $ IntOp size_t) (IntOp i32) (LocInfoE loc_10 (i2v 1 i32))) ;
+        locinfo: loc_8 ;
+        LocInfoE loc_9 ((LocInfoE loc_10 (!{PtrOp} (LocInfoE loc_11 ("ssp")))) at{struct_SolenoidSwitchingParams_t} "state") <-{ IntOp size_t }
+          LocInfoE loc_12 (UnOp (CastOp $ IntOp size_t) (IntOp i32) (LocInfoE loc_12 (i2v 1 i32))) ;
         Return (VOID)
       ]> $
       <[ "#2" :=
@@ -122,31 +131,45 @@ Section code.
   |}.
 
   (* Definition of function [SML_handleReceivedMsgs]. *)
-  Definition impl_SML_handleReceivedMsgs (global_SCH_recieveFullMsg global_SML_switchTheSolenoid : loc): function := {|
+  Definition impl_SML_handleReceivedMsgs (global_SCH_recieveFullMsg : loc): function := {|
     f_args := [
       ("ssp", void*)
     ];
     f_local_vars := [
+      ("rxMsgSize", it_layout u8)
     ];
     f_init := "#0";
     f_code := (
       <[ "#0" :=
-        locinfo: loc_20 ;
-        expr: (LocInfoE loc_20 (Call (LocInfoE loc_36 (global_SCH_recieveFullMsg)) [@{expr} LocInfoE loc_37 (use{PtrOp} (LocInfoE loc_38 ("ssp"))) ])) ;
-        locinfo: loc_29 ;
-        if{IntOp i32}: LocInfoE loc_29 ((LocInfoE loc_30 (use{IntOp size_t} (LocInfoE loc_31 ((LocInfoE loc_32 (!{PtrOp} (LocInfoE loc_33 ("ssp")))) at{struct_SolenoidSwitchingParams_t} "msg")))) ={IntOp size_t, IntOp size_t, i32} (LocInfoE loc_34 (UnOp (CastOp $ IntOp size_t) (IntOp i32) (LocInfoE loc_34 (i2v 8 i32)))))
+        "rxMsgSize" <-{ IntOp u8 }
+          LocInfoE loc_42 (Call (LocInfoE loc_44 (global_SCH_recieveFullMsg)) [@{expr} LocInfoE loc_45 (use{PtrOp} (LocInfoE loc_46 ("ssp"))) ]) ;
+        locinfo: loc_38 ;
+        if{IntOp i32}: LocInfoE loc_38 ((LocInfoE loc_39 (UnOp (CastOp $ IntOp i32) (IntOp u8) (LocInfoE loc_39 (use{IntOp u8} (LocInfoE loc_40 ("rxMsgSize")))))) !={IntOp i32, IntOp i32, i32} (LocInfoE loc_41 (i2v 0 i32)))
         then
-        locinfo: loc_23 ;
+        locinfo: loc_33 ;
           Goto "#1"
         else
-        Goto "#2"
+        Goto "#4"
       ]> $
       <[ "#1" :=
-        locinfo: loc_23 ;
-        expr: (LocInfoE loc_23 (Call (LocInfoE loc_25 (global_SML_switchTheSolenoid)) [@{expr} LocInfoE loc_26 (use{PtrOp} (LocInfoE loc_27 ("ssp"))) ])) ;
-        Return (VOID)
+        locinfo: loc_33 ;
+        if{IntOp i32}: LocInfoE loc_33 ((LocInfoE loc_34 (UnOp (CastOp $ IntOp i32) (IntOp u8) (LocInfoE loc_34 (use{IntOp u8} (LocInfoE loc_35 ("rxMsgSize")))))) ={IntOp i32, IntOp i32, i32} (LocInfoE loc_36 (i2v 8 i32)))
+        then
+        locinfo: loc_27 ;
+          Goto "#2"
+        else
+        Goto "#3"
       ]> $
       <[ "#2" :=
+        locinfo: loc_27 ;
+        LocInfoE loc_28 ((LocInfoE loc_29 (!{PtrOp} (LocInfoE loc_30 ("ssp")))) at{struct_SolenoidSwitchingParams_t} "state") <-{ IntOp size_t }
+          LocInfoE loc_31 (UnOp (CastOp $ IntOp size_t) (IntOp i32) (LocInfoE loc_31 (i2v 1 i32))) ;
+        Return (VOID)
+      ]> $
+      <[ "#3" :=
+        Return (VOID)
+      ]> $
+      <[ "#4" :=
         Return (VOID)
       ]> $∅
     )%E
