src/proofs/funcall/generated_spec.v
@@ -1,0 +1,97 @@
+From refinedc.typing Require Import typing.
+From refinedc.project.learning.src.funcall Require Import generated_code.
+Set Default Proof Using "Type".
+
+(* Generated from [src/funcall.c]. *)
+Section spec.
+  Context `{!typeG Σ} `{!globalG Σ}.
+
+  (* Type definitions. *)
+
+  (* Function [atoi] has been skipped. *)
+
+  (* Function [atol] has been skipped. *)
+
+  (* Function [atoll] has been skipped. *)
+
+  (* Function [atof] has been skipped. *)
+
+  (* Function [strtod] has been skipped. *)
+
+  (* Function [strtof] has been skipped. *)
+
+  (* Function [strtold] has been skipped. *)
+
+  (* Function [strtol] has been skipped. *)
+
+  (* Function [strtoll] has been skipped. *)
+
+  (* Function [strtoul] has been skipped. *)
+
+  (* Function [strtoull] has been skipped. *)
+
+  (* Function [rand] has been skipped. *)
+
+  (* Function [srand] has been skipped. *)
+
+  (* Function [aligned_alloc] has been skipped. *)
+
+  (* Function [calloc] has been skipped. *)
+
+  (* Function [free] has been skipped. *)
+
+  (* Function [malloc] has been skipped. *)
+
+  (* Function [realloc] has been skipped. *)
+
+  (* Function [abort] has been skipped. *)
+
+  (* Function [atexit] has been skipped. *)
+
+  (* Function [at_quick_exit] has been skipped. *)
+
+  (* Function [exit] has been skipped. *)
+
+  (* Function [_Exit] has been skipped. *)
+
+  (* Function [quick_exit] has been skipped. *)
+
+  (* Function [getenv] has been skipped. *)
+
+  (* Function [system] has been skipped. *)
+
+  (* Function [bsearch] has been skipped. *)
+
+  (* Function [qsort] has been skipped. *)
+
+  (* Function [abs] has been skipped. *)
+
+  (* Function [labs] has been skipped. *)
+
+  (* Function [llabs] has been skipped. *)
+
+  (* Function [div] has been skipped. *)
+
+  (* Function [ldiv] has been skipped. *)
+
+  (* Function [lldiv] has been skipped. *)
+
+  (* Function [mblen] has been skipped. *)
+
+  (* Function [mbtowc] has been skipped. *)
+
+  (* Function [wctomb] has been skipped. *)
+
+  (* Function [mbstowcs] has been skipped. *)
+
+  (* Function [wcstombs] has been skipped. *)
+
+  (* Specifications for function [nondent]. *)
+  Definition type_of_nondent :=
+    fn(∀ () : (); True) → ∃ v : bool, (v @ (builtin_boolean)); True.
+
+  (* Specifications for function [foo]. *)
+  Definition type_of_foo :=
+    fn(∀ () : (); True)
+      → ∃ (v, w) : Z * Z, (v @ (int (i32))); ⌜v = 1 ∨ v = 2⌝.
+End spec.
